Fix lean examples

formal-proofs/Aara.lean
@@ -3,70 +3,82 @@ import Mathlib.Tactic.Linarith
 @[simp, reducible]
 abbrev Resource := {r: Int // r ≥ 0}
 
+
 --Needed to instantiate ResourcePairs
 instance : OfNat Resource n where
   ofNat := { val := n, property := by linarith}
 
-structure ResourcePair where
-  --Initial and Residual Resources
-  rp :: (init: Resource) (resid: Resource)
+abbrev ResourcePair := Resource × Resource
 
-open ResourcePair
+--Initial resources
+def ResourcePair.init : ResourcePair → Resource := Prod.fst
+
+--Residual resources
+def ResourcePair.resid : ResourcePair → Resource := Prod.snd 
 
 --Concrete Resource consumption, definition ... in thesis
 @[simp, reducible]
-def ResourcePair.consumption (p : ResourcePair) : Int := p.resid - p.init 
+def ResourcePair.consumption (p : ResourcePair) : Int := p.init - p.resid 
 
 --Resource disparity, definition ... in thesis
 @[simp, reducible]
-def ResourcePair.disparity (p q : ResourcePair) := max p.resid q.init 
+def ResourcePair.disparity (p q : ResourcePair) : Resource := max p.resid q.init 
 
 --Equality of resource pairs
 @[simp, reducible]
 def ResourcePair.equal (p q: ResourcePair) := p.init = q.init ∧ p.consumption = q.consumption
 
+--Neutral element in Resource Pairs
+def ResourcePair.unit := (0, 0)
+
 --Multiplication of resource pairs
 @[simp, reducible]
-def ResourcePair.mult (p q : ResourcePair) := 
-  let r : Resource   := {val := p.init.val - p.resid + p.disparity q, property := by sorry}
-  let r': Resource   := {val := q.resid.val - q.init + p.disparity q, property := by sorry}
-  rp r r'
+def ResourcePair.mult (p q : ResourcePair) : ResourcePair := 
+  let r := {val := p.init.val - p.resid + p.disparity q, property := by sorry}
+  let r':= {val := q.resid.val - q.init + p.disparity q, property := by sorry}
+  (r, r')
 
 -- Relaxation relation
-def ResourcePair.relaxation_of (p q : ResourcePair) : Prop 
-  := p.init ≥ q.init ∧ p.consumption ≥ q.consumption 
+def ResourcePair.relaxation_of (p q : ResourcePair) : Bool 
+  := (p.init ≥ q.init) ∧ (p.consumption ≥ q.consumption) 
 
 infix:50 "≽" => ResourcePair.relaxation_of
 
+infix:50 "⬝" => ResourcePair.mult
+
+
 --Relaxation is partial ordering
 theorem relaxation_reflexive (p : ResourcePair) : p ≽ p := by
-  simp [relaxation_of]
+  simp [ResourcePair.relaxation_of]
 
 theorem relaxation_transitive (p q r: ResourcePair) : p ≽ q → q ≽ r → p ≽ r := by
-  simp [relaxation_of]
+  simp [ResourcePair.relaxation_of]
   intros H_p H_p' H_q H_q'
   apply And.intro
   apply le_trans H_q H_p
   linarith
   
 theorem relaxation_antisymmetric (p q :ResourcePair) : p ≽ q → q ≽ p → p.equal q := by
-  simp [relaxation_of]
+  simp [ResourcePair.relaxation_of]
   intros H_p H_p' H_q H_q'
   apply And.intro
   apply le_antisymm H_q H_p
   linarith
 
+--Example 2.5
+#eval (4, 2) ⬝ (5, 0) -- (7, 0)
+
 --Example 2.7
-#eval true = (rp 4 2 ≽ rp 3 2)
+#eval ((4, 2) ≽ (3, 2))
 
 --Example 2.8
-#eval false = (rp 4 2 ≽ 5 4)
+#eval ((4, 2) ≽ (5, 4))
 
 --Example 2.9
-#eval false = (rp 5 4 ≽ rp 2 0)
+#eval ((5, 4) ≽ (2, 0))
 
 --Example 2.10
-#eval false = (rp 4 2 ≽ rp 5 4) ∧ false = (rp 5 4 ≽ rp 4 2)
+#eval ((4, 2) ≽ (5, 4)) ∧ ((5, 4) ≽ (4, 2))
 
 
 namespace LetTick
@@ -83,9 +95,9 @@ def RAType := BaseType × ResourcePair
 --Evaluation judgement
 inductive Evaluation : Prog → ResourcePair → Prop :=
   | e_tick_pos (k : Int) (pos : k ≥ 0):
-    Evaluation (.tick k) (rp ⟨k, pos⟩ 0) 
+    Evaluation (.tick k) (⟨k, pos⟩, 0) 
   | e_tick_neg (k : Int) (neg: k < 0):
-    Evaluation (.tick (abs k)) (rp ⟨(abs k), abs_nonneg k⟩ 0)
+    Evaluation (.tick (abs k)) (⟨(abs k), abs_nonneg k⟩, 0)
   | e_let {e_1 e_2 : Prog} {r_1 r_2 : ResourcePair} (eval_e_1 : Evaluation e_1 r_1) (eval_e_2 : Evaluation e_2 r_2)
     : Evaluation (.let e_1 e_2) (r_1.mult r_2)
 
@@ -94,7 +106,7 @@ inductive Typing : Prog → BaseType → ResourcePair → Prop :=
   | t_tick (k : Int) (t : BaseType) (r : ResourcePair) (suff_res : r.init ≥ k + r.resid) :
     Typing (.tick k) t r
   | t_let {e_1 e_2 : Prog} {r_1 r_2 : ResourcePair} {t_1 t_2 : BaseType} (e_1types : Typing e_1 t_1 r_1) (e_2Types : Typing e_2 t_2 r_2) (suff_res : r_1.resid = r_2.init) :
-    Typing (.let e_1 e_2) t_2 (rp r_1.init r_2.resid)
+    Typing (.let e_1 e_2) t_2 (r_1.init, r_2.resid)
 
 --Proof of soundness. Theorem 3.5
 theorem soundness (p : Prog) (r_1 r_2 : ResourcePair) (t : BaseType) 
